sheeran1.v
@@ -1,0 +1,145 @@
+Require Import common.
+Require Import Omega.
+
+Set SMT Solver "z3".
+Set SMT Debug.
+
+
+Definition Sheeran_method1 (I : init) (T : trans) (P : prop) (size k: nat) : Prop :=
+  ((lasso I T P size k) \/
+   (violate_loop_free I T P size k)) /\ safety I T P k.
+
+(*
+Tactic Notation "Sheeran_smt_solve1" :=
+ unfold Sheeran_method1;
+ unfold state, lasso, violate_loop_free, safety;
+ unfold loop_free, P_state1;
+ simpl;
+ repeat tryif split then try split else
+     tryif right; intros; smt solve then apply by_smt
+     else  left; intros; smt solve; apply by_smt.
+*)
+
+(*Example Sheeran_method1_test1 :
+  Sheeran_method1 ex_I ex_T ex_P 3 4.
+Proof.
+  unfold ex_I, ex_T, ex_P.
+  unfold Sheeran_method1, lasso, violate_loop_free, safety;
+  split;
+  unfold loop_free, P_state1;
+  unfold state;
+  simpl;
+  unfold neq_state.
+
+  (right; intros; smt solve; apply by_smt) ||
+  (left; intros; smt solve; apply by_smt).
+
+  repeat tryif split then split
+    else smt solve; apply by_smt.
+Qed.
+*)
+
+(* *)
+
+Theorem Sheeran_method_soundness_case1 :
+  forall (I : init) (T : trans) (P : prop) (size k : nat),
+  Sheeran_method1 I T P size k -> 
+    (forall (i : nat), (i <= k) -> P_state2 I T P size i).
+Proof.
+  intros.
+  unfold Sheeran_method1 in H.
+  destruct H.
+  apply (le_safety_relation I T P) in H0.
+  firstorder.
+  auto.
+Qed.
+
+
+Lemma case2_1 :
+  forall (I : init) (T : trans) (P : prop) (size i k : nat),
+  i > k -> lasso I T P size k -> P_state2 I T P size i.
+Proof.
+  unfold lasso, P_state2 in *.
+  intros.
+  apply neg_false.
+  split.
+  intros.
+  destruct H1.
+  destruct H2.
+  assert (H4 : i = k + (i - k)) by omega.
+  rewrite H4 in H2.
+  apply divide_loop_free in H2.
+  firstorder.
+  firstorder.
+Qed.
+
+Theorem case2_2' : forall (T : trans) (P : prop) (size i k : nat),
+  i > k -> 
+  (forall ss : sseq, ~ (loop_free T ss size 0 k /\ ~ P ss.[k])) -> 
+  forall ss : sseq, ~ (loop_free T ss size (i-k) k /\ ~ P ss.[i]).
+Proof.
+  intros.
+  apply neg_false.
+  split.
+  unfold loop_free in *.
+  intros.
+  destruct H1.
+  destruct H1.
+  apply no_loop_skipn_relation in H3.
+  apply P_skipn_relation with (k:= k) in H2.
+  apply path_skipn_relation in H1.
+  firstorder.
+  omega.
+  tauto.
+Qed.
+
+Theorem case2_2 : forall (I : init) (T : trans) (P : prop) (size i k : nat),
+  i > k -> 
+  violate_loop_free I T P size k -> 
+  P_state2 I T P size i.
+Proof.
+  unfold violate_loop_free, P_state2.
+  intros.
+  apply neg_false.
+  split.
+  intros.
+  destruct H1.
+  destruct H2.
+  assert (i = (i - k) + k) by omega.
+  rewrite H4 in H2.
+  apply divide_loop_free in H2.
+  apply case2_2' with (i := i) (k := k) (ss := ss) in H0.
+  firstorder.
+  apply H.
+  tauto.
+Qed.
+
+Theorem Sheeran_method_soundness_case2 :
+  forall (I : init) (T : trans) (P : prop) (size k : nat),
+  Sheeran_method1 I T P size k -> 
+  forall (i : nat), (i > k) -> P_state2 I T P size i.
+Proof.
+  intros.
+  unfold Sheeran_method1 in H.
+  destruct H.
+
+  destruct H.
+  - now apply case2_1 with (k := k).
+
+  - now apply case2_2 with (k := k).
+Qed.
+
+Theorem Sheeran_method_soundness :
+  forall (I : init) (T : trans) (P : prop) (size k : nat),
+  Sheeran_method1 I T P size k -> 
+  forall (i : nat), P_state2 I T P size i.
+Proof.
+  intros.
+  destruct (Nat.le_gt_cases i k).
+  - revert H0.
+    now apply Sheeran_method_soundness_case1.
+  - revert H0.
+    now apply Sheeran_method_soundness_case2.
+Qed.
+
+(* eof *)
